src/equiv/PFtoA.v
@@ -30,43 +30,50 @@ Require Import PromisingArch.equiv.PFtoA4OBW.
 Require Import PromisingArch.equiv.PFtoA4OBR.
 Require Import PromisingArch.equiv.PFtoA4FR.
 Require Import PromisingArch.equiv.PFtoA4Atomic.
+Require Import PromisingArch.equiv.PFtoA4FOB.
+Require Import PromisingArch.equiv.PFtoA4FP.
 Require Import PromisingArch.equiv.PFtoA4SL.
 
 Set Implicit Arguments.
 
 
 Lemma sim_traces_sim_th'_step
-      p trs atrs ws rs covs vexts
+      p trs atrs ws rs fs covs vexts
       m ex
       (STEP: Machine.pf_exec p m)
-      (SIM: sim_traces p m.(Machine.mem) trs atrs ws rs covs vexts)
+      (SIM: sim_traces p m.(Machine.mem) trs atrs ws rs fs covs vexts)
       (PRE: Valid.pre_ex p ex)
       (CO: ex.(Execution.co) = co_gen ws)
       (RF: ex.(Execution.rf) = rf_gen ws rs)
+      (PF: ex.(Execution.pf) = pf_gen ws fs)
       (INTERNAL: acyclic (Execution.internal ex))
       (CO1: Valid.co1 ex)
       (CO2: Valid.co2 ex)
       (RF1: Valid.rf1 ex)
       (RF2: Valid.rf2 ex)
       (RF_WF: Valid.rf_wf ex)
+      (PF1: Valid.pf1 ex)
+      (PF2: Valid.pf2 ex)
       (TR: IdMap.Forall2
              (fun _ tr sl => exists l, tr = (ExecUnit.mk (fst sl) (snd sl) m.(Machine.mem)) :: l)
              trs m.(Machine.tpool))
       (ATR: IdMap.Forall2
               (fun _ atr aeu => exists l, atr = aeu :: l)
               atrs (Valid.aeus PRE)):
-  forall tid tr atr wl rl covl vextl
-    n eu1 eu2 tr' aeu1 aeu2 atr' w1 w2 wl' r1 r2 rl' cov1 cov2 covl' vext1 vext2 vextl'
+  forall tid tr atr wl rl fl covl vextl
+    n eu1 eu2 tr' aeu1 aeu2 atr' w1 w2 wl' r1 r2 rl' f1 f2 fl' cov1 cov2 covl' vext1 vext2 vextl'
     (FIND_TR: IdMap.find tid trs = Some tr)
     (FIND_ATR: IdMap.find tid atrs = Some atr)
     (FIND_WL: IdMap.find tid ws = Some wl)
     (FIND_RL: IdMap.find tid rs = Some rl)
+    (FIND_FL: IdMap.find tid fs = Some fl)
     (FIND_COVL: IdMap.find tid covs = Some covl)
     (FIND_VEXTL: IdMap.find tid vexts = Some vextl)
     (EU: lastn (S n) tr = eu2 :: eu1 :: tr')
     (AEU: lastn (S n) atr = aeu2 :: aeu1 :: atr')
     (WL: lastn (S n) wl = w2 :: w1 :: wl')
     (RL: lastn (S n) rl = r2 :: r1 :: rl')
+    (FL: lastn (S n) fl = f2 :: f1 :: fl')
     (COV: lastn (S n) covl = cov2 :: cov1 :: covl')
     (VEXT: lastn (S n) vextl = vext2 :: vext1 :: vextl')
     (SIM_TH': sim_th' tid m.(Machine.mem) ex (v_gen vexts) eu1 aeu1),
@@ -79,41 +86,48 @@ Proof.
   - eapply sim_traces_sim_th'_ob_read; eauto.
   - eapply sim_traces_sim_th'_fr; eauto.
   - eapply sim_traces_sim_th'_atomic; eauto.
+  - eapply sim_traces_sim_th'_fob; eauto.
+  - eapply sim_traces_sim_th'_fp; eauto.
 Qed.
 
 Lemma sim_traces_sim_th'
-      p trs atrs ws rs covs vexts
+      p trs atrs ws rs fs covs vexts
       m ex
       (STEP: Machine.pf_exec p m)
-      (SIM: sim_traces p m.(Machine.mem) trs atrs ws rs covs vexts)
+      (SIM: sim_traces p m.(Machine.mem) trs atrs ws rs fs covs vexts)
       (PRE: Valid.pre_ex p ex)
       (CO: ex.(Execution.co) = co_gen ws)
       (RF: ex.(Execution.rf) = rf_gen ws rs)
+      (PF: ex.(Execution.pf) = pf_gen ws fs)
       (INTERNAL: acyclic (Execution.internal ex))
       (CO1: Valid.co1 ex)
       (CO2: Valid.co2 ex)
       (RF1: Valid.rf1 ex)
       (RF2: Valid.rf2 ex)
       (RF_WF: Valid.rf_wf ex)
+      (PF1: Valid.pf1 ex)
+      (PF2: Valid.pf2 ex)
       (TR: IdMap.Forall2
              (fun _ tr sl => exists l, tr = (ExecUnit.mk (fst sl) (snd sl) m.(Machine.mem)) :: l)
              trs m.(Machine.tpool))
       (ATR: IdMap.Forall2
               (fun _ atr aeu => exists l, atr = aeu :: l)
               atrs (Valid.aeus PRE)):
-  forall tid tr atr wl rl covl vextl
-    n eu tr' aeu atr' w wl' r rl' cov covl' vext vextl'
+  forall tid tr atr wl rl fl covl vextl
+    n eu tr' aeu atr' w wl' r rl' f fl' cov covl' vext vextl'
     (N: n < length tr)
     (FIND_TR: IdMap.find tid trs = Some tr)
     (FIND_ATR: IdMap.find tid atrs = Some atr)
     (FIND_WL: IdMap.find tid ws = Some wl)
     (FIND_RL: IdMap.find tid rs = Some rl)
+    (FIND_FL: IdMap.find tid fs = Some fl)
     (FIND_COVL: IdMap.find tid covs = Some covl)
     (FIND_VEXTL: IdMap.find tid vexts = Some vextl)
     (EU: lastn (S n) tr = eu :: tr')
     (AEU: lastn (S n) atr = aeu :: atr')
     (WL: lastn (S n) wl = w :: wl')
     (RL: lastn (S n) rl = r :: rl')
+    (FL: lastn (S n) fl = f :: fl')
     (COV: lastn (S n) covl = cov :: covl')
     (VEXT: lastn (S n) vextl = vext :: vextl'),
     sim_th' tid m.(Machine.mem) ex (v_gen vexts) eu aeu.
@@ -151,27 +165,26 @@ Proof.
     exploit sim_trace_sim_th; eauto. intro TH.
     inv x0.
     unfold Machine.init_with_promises in FIND. ss. rewrite IdMap.mapi_spec, STMT in FIND. inv FIND.
-    (* TODO: probably we need to have a lemma for it.. *)
+
+    Ltac inv_po :=
+      repeat match goal with
+             | [H: Execution.po ?a ?b |- _] => inv H; ss; try lia
+      end.
+
     econs; ss.
     - econs; ss. econs. ii. unfold RMap.init. rewrite ? IdMap.gempty. ss.
     - econs; ss.
-      + ii. inv EID. inv REL. inv H1. inv H7. des. inv H7. ss. lia.
-      + ii. inv EID. inv REL. des_union.
-        * inv H1. des. inv H1. des. inv H1. des. inv H1. ss. lia.
-        * inv H1. des. inv H1. des. inv H1. des. inv H1. ss. lia.
-        * inv H6. des. inv H6. des. inv H6. ss. lia.
-        * inv H1. des. inv H1. ss. lia.
-      + ii. inv EID. inv REL. des_union.
-        * inv H6. des. inv H6. des. inv H6. des. inv H6. ss. lia.
-        * inv H6. des. inv H6. des. inv H6. des. inv H6. ss. lia.
-        * inv H1. des. inv H1. ss. lia.
-      + ii. inv EID. inv REL. inv H1. inv H7. ss. lia.
-      + ii. inv EID. inv REL. inv H1. inv H7. ss. lia.
-      + ii. inv EID. inv REL.
-        * inv H1. des. inv H1. ss. lia.
-        * inv H1. des. inv H1. ss. lia.
-      + ii. inv EID. inv REL. inv H1. inv H7. ss. lia.
-      + right. esplits; eauto. ii. inv H1. inv REL. inv H1. inv H7. ss. lia.
+      + ii. inv EID. inv REL. obtac. inv_po.
+      + ii. inv EID. inv REL. obtac. inv_po.
+      + ii. inv EID. inv REL. des_union; obtac; inv_po.
+        obtac. inv_po.
+      + ii. inv EID. inv REL. des_union; obtac; inv_po.
+        obtac. inv_po.
+      + ii. inv EID. inv REL. obtac. inv_po.
+      + ii. inv EID. inv REL. obtac. inv_po.
+      + ii. inv EID. inv REL; inv H1; obtac; inv_po.
+      + ii. inv EID. inv REL; inv H1; obtac; inv_po.
+      + right. esplits; eauto. ii. inv H1. inv REL. obtac. inv_po.
       + i. destruct view; ss. exploit Promises.promises_from_mem_inv; eauto. i. des.
         hexploit sim_traces_ex; try exact SIM.
         all: try rewrite lastn_all; ss.
@@ -194,6 +207,12 @@ Proof.
           { etrans; eauto. }
           { apply List.nth_error_Some. congr. }
         * clear. lia.
+      + ii. inv EID. inv REL. obtac. inv_po.
+      + ii. inv EID. inv REL. obtac; inv_po.
+      + ii. inv EID. inv REL. obtac. inv_po.
+      + ii. inv EID. inv REL. obtac. inv_po.
+    - ii. ss. lia.
+    - ii. ss. lia.
     - ii. ss. lia.
     - ii. ss. lia.
     - ii. ss. lia.
@@ -205,6 +224,7 @@ Proof.
   exploit lastn_S1; try exact AEU; [unguardH LEN; des; lia|i].
   exploit lastn_S1; try exact WL; [unguardH LEN; des; lia|i].
   exploit lastn_S1; try exact RL; [unguardH LEN; des; lia|i].
+  exploit lastn_S1; try exact FL; [unguardH LEN; des; lia|i].
   exploit lastn_S1; try exact COV; [unguardH LEN; des; lia|i].
   exploit lastn_S1; try exact VEXT; [unguardH LEN; des; lia|i].
   subst. exploit sim_trace_lastn; eauto. instantiate (1 := n). i.
@@ -215,25 +235,29 @@ Proof.
   - rewrite AEU, HDATR. ss.
   - rewrite WL, HDWL. ss.
   - rewrite RL, HDRL. ss.
+  - rewrite FL, HDFL. ss.
   - rewrite COV, HDCOVL. ss.
   - rewrite VEXT, HDVEXTL. ss.
 Qed.
 
 Lemma sim_traces_vext_valid
-      p trs atrs ws rs covs vexts
+      p trs atrs ws rs fs covs vexts
       m ex
       (STEP: Machine.pf_exec p m)
-      (SIM: sim_traces p m.(Machine.mem) trs atrs ws rs covs vexts)
+      (SIM: sim_traces p m.(Machine.mem) trs atrs ws rs fs covs vexts)
       (NOPROMISE: Machine.no_promise m)
       (PRE: Valid.pre_ex p ex)
       (CO: ex.(Execution.co) = co_gen ws)
       (RF: ex.(Execution.rf) = rf_gen ws rs)
+      (PF: ex.(Execution.pf) = pf_gen ws fs)
       (INTERNAL: acyclic (Execution.internal ex))
       (CO1: Valid.co1 ex)
       (CO2: Valid.co2 ex)
       (RF1: Valid.rf1 ex)
       (RF2: Valid.rf2 ex)
       (RF_WF: Valid.rf_wf ex)
+      (PF1: Valid.pf1 ex)
+      (PF2: Valid.pf2 ex)
       (TR: IdMap.Forall2
              (fun _ tr sl => exists l, tr = (ExecUnit.mk (fst sl) (snd sl) m.(Machine.mem)) :: l)
              trs m.(Machine.tpool))
@@ -259,7 +283,15 @@ Lemma sim_traces_vext_valid
       (ATOMIC: ex.(Execution.rmw) eid1 eid2)
       (FRE: Execution.fre ex eid1 eid)
       (COE: Execution.coe ex eid eid2),
-      False>>.
+      False>> /\
+  <<FOB:
+    forall eid1 eid2
+      (FOB: Execution.fob ex eid1 eid2),
+      Time.le ((v_gen vexts) eid1) ((v_gen vexts) eid2)>> /\
+  <<FP:
+    forall eid1 eid2
+      (FP: Execution.fp ex eid1 eid2),
+      Time.lt ((v_gen vexts) eid1) ((v_gen vexts) eid2)>>.
 Proof.
   splits; i.
   - destruct eid1 as [tid1 eid1].
@@ -327,13 +359,50 @@ Proof.
     all: try rewrite lastn_all; s; eauto; try lia.
     intro TH'. eapply TH'.(PFtoA3.ATOMIC); eauto.
     apply List.nth_error_Some. congr.
+  - destruct eid1 as [tid1 eid1].
+    destruct eid2 as [tid2 eid2].
+    exploit Execution.fob_flushopt; eauto. intro EID2. inversion EID2.
+    revert EID. unfold Execution.label. s. rewrite PRE.(Valid.LABELS), IdMap.map_spec.
+    generalize (ATR tid2). generalize (SIM tid2). intros X Y; inv X; inv Y; simplify; ss.
+    i. des. subst.
+    exploit sim_trace_last; eauto. i. des. simplify.
+    exploit sim_trace_length; eauto. s. i. des.
+    hexploit sim_traces_sim_th'; eauto.
+    { s. instantiate (1 := length tr'). lia. }
+    all: try rewrite lastn_all; s; eauto; try lia.
+    intro TH'. eapply TH'.(PFtoA3.FOB); eauto.
+    apply List.nth_error_Some. congr.
+  - destruct eid1 as [tid1 eid1].
+    destruct eid2 as [tid2 eid2].
+    dup FP. guardH FP. obtac.
+    + exploit PF2; eauto. i. des. inv PERSIST.
+      revert H2. unfold Execution.label. s. rewrite PRE.(Valid.LABELS), IdMap.map_spec.
+      generalize (ATR tid1). generalize (SIM tid1). intros X Y; inv X; inv Y; simplify; ss.
+      i. des. subst.
+      exploit sim_trace_last; eauto. i. des. simplify.
+      exploit sim_trace_length; eauto. s. i. des.
+      hexploit sim_traces_sim_th'; eauto.
+      { s. instantiate (1 := length tr'). lia. }
+      all: try rewrite lastn_all; s; eauto; try lia.
+      intro TH'. eapply TH'.(PFtoA3.FP); eauto.
+      apply List.nth_error_Some. congr.
+    + revert EID1. unfold Execution.label. s. rewrite PRE.(Valid.LABELS), IdMap.map_spec.
+      generalize (ATR tid1). generalize (SIM tid1). intros Z W. inv Z; inv W; simplify; ss.
+      i. des. subst.
+      exploit sim_trace_last; eauto. i. des. simplify.
+      exploit sim_trace_length; eauto. s. i. des.
+      hexploit sim_traces_sim_th'; eauto.
+      { s. instantiate (1 := length tr'). lia. }
+      all: try rewrite lastn_all; s; eauto; try lia.
+      intro TH'. eapply TH'.(PFtoA3.FP); eauto.
+      apply List.nth_error_Some. congr.
 Qed.
 
 Lemma sim_traces_valid_internal
-      p trs atrs ws rs covs vexts
+      p trs atrs ws rs fs covs vexts
       m ex
       (STEP: Machine.pf_exec p m)
-      (SIM: sim_traces p m.(Machine.mem) trs atrs ws rs covs vexts)
+      (SIM: sim_traces p m.(Machine.mem) trs atrs ws rs fs covs vexts)
       (PRE: Valid.pre_ex p ex)
       (CO: ex.(Execution.co) = co_gen ws)
       (RF: ex.(Execution.rf) = rf_gen ws rs)
@@ -375,19 +444,22 @@ Proof.
 Qed.
 
 Lemma sim_traces_valid_external_atomic
-      p trs atrs ws rs covs vexts
+      p trs atrs ws rs fs covs vexts
       m ex
       (STEP: Machine.pf_exec p m)
-      (SIM: sim_traces p m.(Machine.mem) trs atrs ws rs covs vexts)
+      (SIM: sim_traces p m.(Machine.mem) trs atrs ws rs fs covs vexts)
       (PRE: Valid.pre_ex p ex)
       (CO: ex.(Execution.co) = co_gen ws)
       (RF: ex.(Execution.rf) = rf_gen ws rs)
+      (PF: ex.(Execution.pf) = pf_gen ws fs)
       (INTERNAL: acyclic (Execution.internal ex))
       (CO1: Valid.co1 ex)
       (CO2: Valid.co2 ex)
       (RF1: Valid.rf1 ex)
       (RF2: Valid.rf2 ex)
       (RF_WF: Valid.rf_wf ex)
+      (PF1: Valid.pf1 ex)
+      (PF2: Valid.pf2 ex)
       (TR: IdMap.Forall2
              (fun _ tr sl => exists l, tr = (ExecUnit.mk (fst sl) (snd sl) m.(Machine.mem)) :: l)
              trs m.(Machine.tpool))
@@ -397,27 +469,168 @@ Lemma sim_traces_valid_external_atomic
   <<EXTERNAL:
     forall eid1 eid2
       (OB: Execution.ob ex eid1 eid2)
-      (LABEL1: Execution.label_is ex Label.is_access eid1)
-      (LABEL2: Execution.label_is ex Label.is_access eid2),
+      (LABEL1: Execution.label_is ex Label.is_access_persist eid1)
+      (LABEL2: Execution.label_is ex Label.is_access_persist eid2),
       (Time.lt ((v_gen vexts) eid1) ((v_gen vexts) eid2) /\ ex.(Execution.label_is) Label.is_write eid2) \/
-      (Time.le ((v_gen vexts) eid1) ((v_gen vexts) eid2) /\ ex.(Execution.label_is) Label.is_read eid2)>> /\
+      (Time.le ((v_gen vexts) eid1) ((v_gen vexts) eid2) /\ ex.(Execution.label_is) Label.is_read eid2) \/
+      (Time.le ((v_gen vexts) eid1) ((v_gen vexts) eid2) /\ ex.(Execution.label_is) Label.is_flushopt eid2)>> /\
   <<ATOMIC: le (ex.(Execution.rmw) ∩ ((Execution.fre ex) ⨾ (Execution.coe ex))) bot>>.
 Proof.
   generalize STEP. intro X. inv X. splits.
   - exploit sim_traces_vext_valid; eauto. i. des.
     inv LABEL2. destruct l; ss.
-    + right. rewrite ob_ob' in OB. des_union.
-      * exploit FR; eauto. i.
-        split; eauto using Nat.lt_le_incl.
-      * exploit sim_traces_vext_co; eauto. i.
-        split; eauto using Nat.lt_le_incl.
-      * exploit OB_READ; eauto.
-    + left. rewrite ob_ob' in OB. des_union.
-      * exploit FR; eauto.
+    + right. left. rewrite ob_ob' in OB. des_union; eauto.
+      * obtac; cycle 1.
+        { destruct l; ss. congr. }
+        exploit CO2; eauto. i. des. congr.
+      * exploit CO2; eauto. i. des. congr.
+      * obtac; cycle 1.
+        { destruct l; ss. congr. }
+        exploit CO2; eauto. i. des. congr.
+    + left. rewrite ob_ob' in OB. des_union; eauto.
       * exploit sim_traces_vext_co; eauto.
-      * exploit OB_WRITE; eauto.
+      * exploit Execution.fob_flushopt; eauto. intro Z. inv Z.
+        destruct l; ss. congr.
+    + repeat right. rewrite ob_ob' in OB. des_union; eauto.
+      * obtac; cycle 1.
+        { destruct l; ss. congr. }
+        exploit CO2; eauto. i. des. congr.
+      * exploit CO2; eauto. i. des. congr.
+      * obtac; cycle 1.
+        { destruct l; ss. congr. }
+        exploit CO2; eauto. i. des. congr.
+      * exfalso. eapply ob'_flushopt; eauto.
   - exploit sim_traces_vext_valid; eauto. i. des.
     ii. inv H. inv H1. des. exfalso. eauto.
+Qed.
+
+Lemma sim_traces_valid_per
+      p trs atrs ws rs fs covs vexts
+      m ex smem
+      (STEP: Machine.pf_exec p m)
+      (PMEM: Machine.persisted m smem)
+      (SIM: sim_traces p m.(Machine.mem) trs atrs ws rs fs covs vexts)
+      (NOPROMISE: Machine.no_promise m)
+      (PRE: Valid.pre_ex p ex)
+      (CO: ex.(Execution.co) = co_gen ws)
+      (RF: ex.(Execution.rf) = rf_gen ws rs)
+      (PF: ex.(Execution.pf) = pf_gen ws fs)
+      (INTERNAL: acyclic (Execution.internal ex))
+      (CO1: Valid.co1 ex)
+      (CO2: Valid.co2 ex)
+      (RF1: Valid.rf1 ex)
+      (RF2: Valid.rf2 ex)
+      (RF_WF: Valid.rf_wf ex)
+      (PF1: Valid.pf1 ex)
+      (PF2: Valid.pf2 ex)
+      (TR: IdMap.Forall2
+             (fun _ tr sl => exists l, tr = (ExecUnit.mk (fst sl) (snd sl) m.(Machine.mem)) :: l)
+             trs m.(Machine.tpool))
+      (ATR: IdMap.Forall2
+              (fun _ atr aeu => exists l, atr = aeu :: l)
+              atrs (Valid.aeus PRE)):
+  forall eid loc
+    (EID: ex.(Execution.label_is) (Label.is_writing loc) eid)
+    (DOM: dom_rel (Execution.per ex) eid),
+    exists tid sl msg,
+      <<SL: IdMap.find tid m.(Machine.tpool) = Some sl>> /\
+      <<MSG: Memory.get_msg ((v_gen vexts) eid) m.(Machine.mem) = Some msg>> /\
+      msg.(Msg.loc) = loc /\
+      Time.le ((v_gen vexts) eid) ((snd sl).(Local.per) loc).(View.ts).
+Proof.
+  i. destruct eid as [tid iid]. obtac.
+  generalize EID0. unfold Execution.label. s. rewrite PRE.(Valid.LABELS), IdMap.map_spec.
+  generalize (ATR tid). generalize (SIM tid). intros X Y; inv X; inv Y; simplify; ss.
+  i. des. subst.
+  generalize (TR tid). intro X. inv X; simplify. destruct b as [st lc].
+  exploit sim_trace_last; eauto. i. des. simplify.
+  exploit sim_trace_length; eauto. s. i. des.
+  hexploit sim_trace_sim_th; eauto; ss. intro L.
+  move EID0 at bottom. destruct l; ss. eqvtac.
+  exploit L.(WPROP2); eauto. i. des.
+  exploit L.(WPROP3); eauto. i. des. subst.
+  move DOM at bottom. inv DOM. obtac.
+
+  exploit PF2; eauto. i. des. obtac.
+  rewrite PERSIST in EID. rewrite WRITE in EID0. simplify.
+  destruct x8 as [ftid0 fiid]. destruct x as [ftid fiid1].
+  generalize H11. intro Z. inv Z. ss. subst.
+  generalize EID2. unfold Execution.label. s. rewrite PRE.(Valid.LABELS), IdMap.map_spec.
+  generalize (ATR ftid). generalize (SIM ftid). intros Z W; inv Z; inv W; simplify; ss.
+  i. des. subst.
+  generalize (TR ftid). intro Z. inv Z; simplify. destruct b as [st0 lc0]. ss.
+  symmetry in H20. esplits; try exact H20; eauto; s.
+  { unfold v_gen. s. rewrite <- H6. rewrite x4. eauto. }
+  { ss. }
+
+  exploit sim_traces_vext_pf; eauto. etrans; eauto.
+  exploit sim_trace_last; eauto. i. des. simplify.
+  exploit sim_trace_length; eauto. s. i. des.
+  hexploit sim_traces_sim_th'; eauto.
+  { s. instantiate (1 := length tr'0). lia. }
+  all: try rewrite lastn_all; s; eauto; try lia.
+  intro TH'.
+  eapply TH'.(LC).(PER_END). econs; eauto.
+  econs. simtac.
+  econs; eauto. apply List.nth_error_Some. ss. rewrite EID0. ss.
+Qed.
+
+Lemma sim_traces_persisted
+      p trs atrs ws rs fs covs vexts
+      m ex smem
+      (STEP: Machine.pf_exec p m)
+      (PMEM: Machine.persisted m smem)
+      (SIM: sim_traces p m.(Machine.mem) trs atrs ws rs fs covs vexts)
+      (NOPROMISE: Machine.no_promise m)
+      (PRE: Valid.pre_ex p ex)
+      (CO: ex.(Execution.co) = co_gen ws)
+      (RF: ex.(Execution.rf) = rf_gen ws rs)
+      (PF: ex.(Execution.pf) = pf_gen ws fs)
+      (INTERNAL: acyclic (Execution.internal ex))
+      (CO1: Valid.co1 ex)
+      (CO2: Valid.co2 ex)
+      (RF1: Valid.rf1 ex)
+      (RF2: Valid.rf2 ex)
+      (RF_WF: Valid.rf_wf ex)
+      (PF1: Valid.pf1 ex)
+      (PF2: Valid.pf2 ex)
+      (TR: IdMap.Forall2
+             (fun _ tr sl => exists l, tr = (ExecUnit.mk (fst sl) (snd sl) m.(Machine.mem)) :: l)
+             trs m.(Machine.tpool))
+      (ATR: IdMap.Forall2
+              (fun _ atr aeu => exists l, atr = aeu :: l)
+              atrs (Valid.aeus PRE)):
+  Valid.persisted ex smem.
+Proof.
+  ii. generalize (PMEM loc). intro X. inv X.
+  exploit Memory.read_get_msg; eauto. i. des.
+  - econs; eauto. i. inversion PEID.
+    exploit sim_traces_valid_per; eauto. i. des.
+    specialize (LATEST tid sl). eapply LATEST in SL.
+    unfold Memory.get_msg in MSG. destruct (v_gen vexts eid); ss. eapply SL; try exact MSG; eauto.
+    subst. unfold Time.bot. lia.
+  - exploit sim_traces_memory; eauto. i. des.
+    generalize (SIM tid). intro X. inv X; simplify.
+    generalize (TR tid). intro X. inv X; simplify.
+    generalize (ATR tid). intro X. inv X; simplify.
+    exploit sim_trace_last; eauto. i. des.
+    exploit sim_trace_length; eauto. s. i. des. subst; ss.
+    hexploit sim_trace_sim_th; eauto. simplify. intro L.
+    exploit L.(WPROP1); eauto. i. des.
+    { symmetry in H7. destruct b0 as [st0 lc0]. ss.
+      inv NOPROMISE. eapply PROMISES in H7.
+      rewrite H7 in x2. rewrite Promises.lookup_bot in x2. ss.
+    }
+    exploit L.(WPROP3); eauto. i. des. subst.
+    econs 2.
+    { instantiate (3 := (tid, eid)). unfold Execution.label. s.
+      rewrite PRE.(Valid.LABELS), IdMap.map_spec, <- H8. ss. eauto.
+    }
+    i. exploit sim_traces_vext_co; eauto; try by (subst; ss). i.
+    inv PEID. exploit sim_traces_valid_per; eauto. i. des.
+    move LATEST at bottom. eapply LATEST in SL.
+    unfold Memory.get_msg in MSG. destruct (v_gen vexts eid2); ss. eapply SL; try exact MSG; eauto.
+    unfold v_gen in *. ss. rewrite <- H6 in *. rewrite x7 in x6. unfold Time.lt in *. ss.
 Qed.
 
 Lemma internal_acyclic
@@ -440,14 +653,17 @@ Proof.
 Qed.
 
 Lemma promising_pf_valid
-      p m
-      (STEP: Machine.pf_exec p m):
+      p m smem
+      (STEP: Machine.pf_exec p m)
+      (PMEM: Machine.persisted m smem):
   exists ex (PRE: Valid.pre_ex p ex) (cov: forall (eid: eidT), Time.t) (vext: forall (eid: eidT), Time.t),
     <<CO1: Valid.co1 ex>> /\
     <<CO2: Valid.co2 ex>> /\
     <<RF1: Valid.rf1 ex>> /\
     <<RF2: Valid.rf2 ex>> /\
     <<RF_WF: Valid.rf_wf ex>> /\
+    <<PF1: Valid.pf1 ex>> /\
+    <<PF2: Valid.pf2 ex>> /\
     <<INTERNAL:
       forall eid1 eid2
         (INTERNAL: (Execution.internal ex)⁺ eid1 eid2),
@@ -461,23 +677,25 @@ Lemma promising_pf_valid
          ex.(Execution.label_is) Label.is_read eid2)>> /\
     <<EXTERNAL:
       forall eid1 eid2
-        (OB: (Execution.ob ex ∩ (ex.(Execution.label_is_rel) Label.is_access))⁺ eid1 eid2),
+        (OB: (Execution.ob ex ∩ (ex.(Execution.label_is_rel) Label.is_access_persist))⁺ eid1 eid2),
         Time.lt (vext eid1) (vext eid2) \/
         (Time.le (vext eid1) (vext eid2) /\
-         Execution.po eid1 eid2 /\
-         ex.(Execution.label_is) Label.is_read eid1 /\
-         ex.(Execution.label_is) Label.is_read eid2) \/
-        (Time.le (vext eid1) (vext eid2) /\
-         ex.(Execution.label_is) Label.is_write eid1 /\
-         ex.(Execution.label_is) Label.is_read eid2)>> /\
+         ((Execution.po eid1 eid2 /\
+           ex.(Execution.label_is) Label.is_read eid1 /\
+           ex.(Execution.label_is) Label.is_read eid2) \/
+          (ex.(Execution.label_is) Label.is_write eid1 /\
+           ex.(Execution.label_is) Label.is_read eid2) \/
+          (ex.(Execution.label_is) Label.is_access eid1 /\
+           ex.(Execution.label_is) Label.is_flushopt eid2)))>> /\
     <<ATOMIC: le (ex.(Execution.rmw) ∩ ((Execution.fre ex) ⨾ (Execution.coe ex))) bot>> /\
     <<STATE: IdMap.Forall2
                (fun tid sl aeu => sim_state_weak (fst sl) aeu.(AExecUnit.state))
-               m.(Machine.tpool) PRE.(Valid.aeus)>>.
+               m.(Machine.tpool) PRE.(Valid.aeus)>> /\
+    <<PMEM: Valid.persisted ex smem>>.
 Proof.
   exploit promising_pf_sim_traces; eauto. i. des.
   destruct PRE, ex. ss.
-  remember (Execution.mk labels addr data ctrl0 rmw (co_gen ws) (rf_gen ws rs)) as ex'.
+  remember (Execution.mk labels addr data ctrl0 rmw (co_gen ws) (rf_gen ws rs) (pf_gen ws fs)) as ex'.
   replace labels with ex'.(Execution.labels) in LABELS; [|subst; ss].
   replace addr with ex'.(Execution.addr) in ADDR; [|subst; ss].
   replace data with ex'.(Execution.data) in DATA; [|subst; ss].
@@ -492,8 +710,11 @@ Proof.
   generalize (sim_traces_rf1 STEP PRE' NOPROMISE SIM TR ATR). intro RF1.
   generalize (sim_traces_rf2 PRE' SIM ATR). intro RF2.
   generalize (sim_traces_rf_wf SIM). intro RF_WF.
+  generalize (sim_traces_pf1 STEP PRE' NOPROMISE SIM TR ATR). intro PF1.
+  generalize (sim_traces_pf2 STEP PRE' SIM TR ATR). intro PF2.
   replace (co_gen ws) with (ex'.(Execution.co)) in CO1, CO2;[|subst; ss].
   replace (rf_gen ws rs) with (ex'.(Execution.rf)) in RF1, RF2, RF_WF; [|subst; ss].
+  replace (pf_gen ws fs) with (ex'.(Execution.pf)) in PF1, PF2; [|subst; ss].
   hexploit sim_traces_valid_internal; eauto; try by (subst; ss). intro INTERNAL.
   assert (INTERNAL': forall eid1 eid2 (INTERNAL: (Execution.internal ex')⁺ eid1 eid2),
              Time.lt (v_gen covs eid1) (v_gen covs eid2) \/
@@ -534,27 +755,33 @@ Proof.
   esplits; eauto.
   - clear INTERNAL'. i. induction OB.
     + inversion H. inversion H1.
-      exploit EXTERNAL; eauto. i. des; eauto.
-      { destruct l1.
-        - exploit Valid.ob_read_read_po; eauto. i.
-          right. left. splits; eauto.
-        - right. right. splits; eauto.
-        - inv LABEL1.
-        - inv LABEL1.
-        - inv LABEL1.
+      exploit EXTERNAL; eauto. i. des; eauto; cycle 1.
+      { right. exploit Valid.ob_persist_spec; eauto. i. des. eauto. }
+      right. splits; eauto.
+      inversion x1. destruct l; ss.
+      destruct (Label.is_flushopt l1) eqn:LAB.
+      { exploit Valid.persist_ob_write; eauto with axm. intro WR. inversion WR.
+        destruct l; ss; congr.
       }
+      destruct l1; ss; [left|right]; splits; eauto with axm.
+      eapply Valid.ob_read_read_po; eauto with axm.
     + des.
+      all: try by left; eapply le_lt_trans; eauto.
+      all: try by left; eapply lt_le_trans; eauto.
+      all: try by right; split; try etrans; eauto.
       * left. etrans; eauto.
-      * left. eapply le_lt_trans; eauto.
-      * left. eapply le_lt_trans; eauto.
-      * left. eapply lt_le_trans; eauto.
-      * right. left. splits; try etrans; eauto.
-      * right. right. splits; try etrans; eauto.
-      * left. eapply lt_le_trans; eauto.
-      * inversion IHOB6. inversion IHOB0. rewrite EID in EID0.
-        inversion EID0. rewrite H0 in *. ss. destruct l0; ss; congr.
-      * inversion IHOB5. inversion IHOB0. rewrite EID in EID0.
-        inversion EID0. rewrite H0 in *. ss. destruct l0; ss; congr.
+      * right. split; try etrans; eauto.
+        left. simtac. rewrite <- IHOB0. ss.
+      * inversion IHOB3. inversion IHOB6.
+        rewrite EID in EID0. inversion EID0. rewrite H0 in *. destruct l0; ss.
+      * inversion IHOB0. inversion IHOB6.
+        rewrite EID in EID0. inversion EID0. rewrite H0 in *. destruct l0; ss.
+      * inversion IHOB0. inversion IHOB5.
+        rewrite EID in EID0. inversion EID0. rewrite H0 in *. destruct l0; ss.
+      * right. split; try etrans; eauto.
+        right. right. inversion IHOB5. split; simtac.
+      * right. split; try etrans; eauto.
+        right. right. inversion IHOB4. split; simtac.
   - clear - SIM TR ATR.
     ii. generalize (SIM id). i. inv H; ss.
     + generalize (TR id). i. inv H; try congr.
@@ -562,24 +789,28 @@ Proof.
       econs.
     + generalize (TR id). i. inv H; try congr.
       generalize (ATR id). i. inv H; try congr.
-      des. simplify. inv REL6; auto.
+      des. simplify. inv REL7; auto.
       { econs. unfold Machine.init_with_promises in *. ss.
         rewrite IdMap.mapi_spec in *. rewrite STMT in FIND. ss.
         symmetry in FIND. inv FIND. rewrite H0.
         apply sim_state_weak_init. }
+  - (* PMEM *)
+    hexploit sim_traces_persisted; eauto; try by (subst; ss).
 Qed.
 
 Theorem promising_pf_to_axiomatic
-        p m
-        (STEP: Machine.pf_exec p m):
+        p m smem
+        (STEP: Machine.pf_exec p m)
+        (PMEM: Machine.persisted m smem):
   exists ex (EX: Valid.ex p ex),
     <<TERMINAL: Machine.is_terminal m -> Valid.is_terminal EX>> /\
     <<STATE: IdMap.Forall2
                (fun tid sl aeu => sim_state_weak (fst sl) aeu.(AExecUnit.state))
-               m.(Machine.tpool) EX.(Valid.aeus)>>.
+               m.(Machine.tpool) EX.(Valid.aeus)>> /\
+    <<PMEM: Valid.persisted ex smem>>.
 Proof.
   exploit promising_pf_valid; eauto. i. des.
-  exists ex. eexists (Valid.mk_ex PRE CO1 CO2 RF1 RF2 RF_WF _ _ ATOMIC).
+  exists ex. eexists (Valid.mk_ex PRE CO1 CO2 RF1 RF2 RF_WF PF1 PF2 _ _ ATOMIC).
   s. esplits; eauto.
   ii. inv H. specialize (STATE tid). inv STATE; try congr.
   rewrite FIND in H. inv H. destruct a. destruct aeu. ss.
@@ -591,7 +822,8 @@ Grab Existential Variables.
   exploit EXTERNAL; eauto. i. des.
   - inv x; lia.
   - inv x0. lia.
-  - inv x0. inv x1. rewrite EID in EID0. inv EID0. destruct l0; ss; congr.
+  - obtac. destruct l; destruct l0; ss; congr.
+  - obtac. destruct l; destruct l0; ss; congr.
 }
 { (* internal *)
   clear - INTERNAL.
@@ -600,13 +832,15 @@ Grab Existential Variables.
 Qed.
 
 Theorem promising_to_axiomatic
-        p m
-        (STEP: Machine.exec p m):
+        p m smem
+        (STEP: Machine.exec p m)
+        (PMEM: Machine.persisted m smem):
   exists ex (EX: Valid.ex p ex),
     <<TERMINAL: Machine.is_terminal m -> Valid.is_terminal EX>> /\
     <<STATE: IdMap.Forall2
                (fun tid sl aeu => sim_state_weak (fst sl) aeu.(AExecUnit.state))
-               m.(Machine.tpool) EX.(Valid.aeus)>>.
+               m.(Machine.tpool) EX.(Valid.aeus)>> /\
+    <<PMEM: Valid.persisted ex smem>>.
 Proof.
   apply promising_to_promising_pf in STEP.
   apply promising_pf_to_axiomatic; auto.
